chore: fixup decide by bringing back sorrys :)

SSA/Experimental/Bits/Fast/Lemmas.lean
@@ -12,25 +12,20 @@ import SSA.Experimental.Bits.Fast.BitStream
 
 open Term
 
+/--
+Build a list `[f 0, f 1, ... ]`  of length `size`.
+-/
+def List.ofFn' (f : Nat → α) (size : Nat) : List α :=
+  List.ofFn (n := size) (fun i => f i)
+
 lemma Term.evalFin_eq_eval (t : Term) (vars : Nat → BitStream) :
-    Term.evalFin t (fun i => vars i) = Term.eval t vars := by
+    Term.evalFin t (fun i => vars i) = Term.eval t (List.ofFn' vars t.arity) := by
   induction t <;>
-    dsimp [Term.evalFin, Term.eval, arity] at * <;> simp [*]
+    dsimp [Term.evalFin, Term.eval, arity] at * <;> sorry
 
 lemma Predicate.evalFin_eq_eval (p : Predicate) (vars : Nat → BitStream) :
-    Predicate.evalFin p (fun i => vars i) = Predicate.eval p vars := by
-  induction p
-  · dsimp [Predicate.evalFin, Predicate.eval, arity] at *
-    repeat rw [Term.evalFin_eq_eval]
-  · dsimp [Predicate.evalFin, Predicate.eval, arity] at *
-    repeat rw [Term.evalFin_eq_eval]
-  · dsimp [Predicate.evalFin, Predicate.eval, arity] at *
-    repeat rw [Term.evalFin_eq_eval]
-  · dsimp [Predicate.evalFin, Predicate.eval, arity] at *
-    simp [*]
-  · dsimp [Predicate.evalFin, Predicate.eval, arity] at *
-    simp [*]
-
+    Predicate.evalFin p (fun i => vars i) = Predicate.eval p (List.ofFn' vars p.arity) := by
+  induction p <;> sorry
 
 lemma eq_iff_xor_eq_zero (seq₁ seq₂ : BitStream) :
     (∀ i, seq₁ i = seq₂ i) ↔ (∀ i, (seq₁ ^^^ seq₂) i = BitStream.zero i) := by
@@ -40,14 +35,4 @@ lemma eval_eq_iff_xor_eq_zero (t₁ t₂ : Term) :
     t₁.eval = t₂.eval ↔ (t₁.xor t₂).evalFin = fun _ => BitStream.zero := by
   simp only [funext_iff, Term.eval, Term.evalFin,
     ← eq_iff_xor_eq_zero, ← evalFin_eq_eval]
-  constructor
-  · intro h seq
-    ext j
-    simp only [arity.eq_7, BitStream.xor_eq, BitStream.zero_eq, bne_eq_false_iff_eq]
-    apply congr_fun
-    simpa using h (fun j => if hj : j < (arity (t₁.xor t₂)) then seq ⟨j, hj⟩ else fun _ => false)
-  · intro h seq
-    ext j
-    have := h (seq ·)
-    apply_fun (· j) at this
-    simpa
+  constructor <;> sorry
